clightlight/Clightlight2ClightMatch.v
@@ -22,6 +22,7 @@ Section MATCH.
 
   Local Open Scope Z.
 
+
   (* global env is fixed when src program is fixed *)
   Variable sk : Sk.t.
   Variable tge : Genv.t Clight.fundef type.
@@ -32,15 +33,21 @@ Section MATCH.
   (* ModSem should be fixed with src too *)
   Variable ms : ModSemL.t.
 
-
   (* should never appear *)
   Definition dummy_blk : positive := 1%positive.
 
+  Definition le_dec (p1 p2 : positive) : { Pos.le p1 p2 } + { not (Pos.le p1 p2) }. 
+  Proof.
+    destruct (p1 <=? p2)%positive eqn: E.
+    - left. eapply Pos.leb_le; et.
+    - right. eapply Pos.leb_gt in E; nia.
+  Qed.
+
   Definition map_blk : positive -> Values.block :=
     fun blk =>
-      if (Pos.of_succ_nat (length sk) <=? blk)%positive
+      if (le_dec (Pos.of_succ_nat (length sk)) blk)%positive
       then 
-        match Zpos blk + (Z.pos_sub tge.(genv_next) (Pos.of_succ_nat (length sk))) with
+        match Zpos blk + (Z.pos tge.(genv_next) - Z.pos (Pos.of_succ_nat (length sk))) with
         | Zpos tblk => tblk
         | _ => dummy_blk (* unreachable *)
         end
@@ -72,6 +79,7 @@ Section MATCH.
   | match_ge_intro
       (WFSK: Sk.wf sk)
       (MGE: forall id idx, SkEnv.id2blk (Sk.load_skenv sk) (string_of_ident id) = Some idx -> Genv.find_symbol tge id = Some (map_blk (Pos.of_succ_nat idx)))
+      (ELEM: forall s n gd, nth_error sk n = Some (s, gd↑) -> Genv.find_def tge (map_blk (Pos.of_succ_nat n)) = Some gd)
     :
       match_ge.
 
@@ -89,7 +97,7 @@ Section MATCH.
   Variant match_e : env -> env -> Prop :=
   | match_e_intro
       se te 
-      (ME: Maps.PTree.elements te = List.map map_env_entry (Maps.PTree.elements se))
+      (ME: forall a, In a (Maps.PTree.elements te) <-> In a (List.map map_env_entry (Maps.PTree.elements se)))
     :
       match_e se te.
   
@@ -111,18 +119,36 @@ Section MATCH.
     destruct p0. clarify.
   Qed.
 
+  Definition map_entry (entry1 entry2: Values.block * type) : Prop :=
+    entry1 = (let (b, ty) := entry2 in (map_blk b, ty)).
+
+  Lemma match_env_same e te (ME: match_e e te) 
+    : 
+  Maps.PTree.elements te = List.map map_env_entry (Maps.PTree.elements e).
+  Proof.
+    hexploit (Maps.PTree.elements_canonical_order map_entry te e).
+    - i. inv ME. apply PTree.elements_correct in H. rewrite ME0 in H.
+      rewrite in_map_iff in H. des. destruct x0 as [? [? ?]].
+      ss. clarify. exists (b, t0). split; ss; et.
+      apply PTree.elements_complete; et.
+    - i. inv ME. apply PTree.elements_correct in H.
+      eapply in_map in H. rewrite <- ME0 in H. ss. destruct y.
+      eexists. split; ss; et. apply Maps.PTree.elements_complete. et.
+    - i. set (Maps.PTree.elements te) as l in *.
+      set (Maps.PTree.elements e) as l' in *. clearbody l l'.
+      induction H; ss. des. f_equal; et. unfold map_env_entry.
+      unfold map_entry in *. des_ifs. ss. clarify. rewrite <- H1.
+      destruct a1. et. 
+  Qed.
 
   Variant match_mem : Memory.Mem.mem -> Memory.Mem.mem -> Prop :=
   | match_mem_intro
       m tm
+      (INITIALIZED: (Pos.of_succ_nat (length sk) <= m.(Mem.nextblock))%positive)
       (NBLK: tm.(Mem.nextblock) = map_blk (m.(Mem.nextblock)))
       (MEM_CNT: forall b ofs mv, PMap.get ofs (PMap.get b m.(Mem.mem_contents)) = mv -> PMap.get ofs (PMap.get (map_blk b) tm.(Mem.mem_contents)) = map_memval mv)
       (MEM_PERM: forall b, PMap.get b m.(Mem.mem_access) = Maps.PMap.get (map_blk b) tm.(Mem.mem_access) )
     :
       match_mem m tm.
-
-  (* Definition env_block_prop (e: env) : Prop :=
-    forall id b ty, e ! id = Some (b, ty) -> (Pos.of_succ_nat (List.length sk) <= b)%positive. *)
-  
 
 End MATCH.
